theories/typing/bitfield.v
@@ -265,8 +265,8 @@ Section programs.
 
   Lemma type_if_bitfield_raw it n v T1 T2:
     case_if (n ≠ 0)
-      (li_trace (DestructHintIfInt n, true) T1)
-      (li_trace (DestructHintIfInt n, false) T2)
+      (li_trace (TraceIfInt n, true) T1)
+      (li_trace (TraceIfInt n, false) T2)
     ⊢ typed_if (IntOp it) v (v ◁ᵥ n @ bitfield_raw it) T1 T2.
   Proof. unfold bitfield_raw; simpl_type. apply type_if_int. Qed.
   Definition type_if_bitfield_raw_inst := [instance type_if_bitfield_raw].
